set up perf testing for the original itp

theories/interpreter_func.v
@@ -521,3 +521,65 @@ Fixpoint run_v (fuel : fuel) (d : depth) (cfg : config_tuple) : ((host_state * s
   end.
 
 End Host_func.
+
+Module EmptyHost.
+
+Definition host_function := void.
+
+Definition host_function_eq_dec : forall f1 f2 : host_function, {f1 = f2} + {f1 <> f2}.
+Proof. decidable_equality. Defined.
+
+Definition host_function_eqb f1 f2 : bool := host_function_eq_dec f1 f2.
+Definition host_functionP : Equality.axiom host_function_eqb :=
+  eq_dec_Equality_axiom host_function_eq_dec.
+
+Canonical Structure host_function_eqMixin := EqMixin host_functionP.
+Canonical Structure host_function_eqType :=
+  Eval hnf in EqType host_function host_function_eqMixin.
+
+Definition host : Type := host host_function_eqType.
+
+Definition store_record := store_record host_function_eqType.
+Definition function_closure := function_closure host_function_eqType.
+
+Definition host_instance : host.
+Proof.
+  by refine {|
+      host_state := unit_eqType ;
+      host_application _ _ _ _ _ _ _ := False
+    |}; intros; exfalso; auto.
+Defined.
+
+Definition config_tuple := config_tuple host_instance.
+Definition res_tuple := res_tuple host_instance.
+
+Definition host_state := host_state host_instance.
+
+End EmptyHost.
+
+Module Interpreter_func.
+
+Export EmptyHost.
+
+Definition host_application_impl : host_state -> store_record -> function_type -> host_function_eqType -> seq value ->
+                                   (host_state * option (store_record * result)).
+Proof.
+  move => ??? hf; by inversion hf.
+Defined.
+
+Definition host_application_impl_correct :
+  (forall hs s ft hf vs hs' hres, (host_application_impl hs s ft hf vs = (hs', hres)) -> host_application hs s ft hf vs hs' hres).
+Proof.
+  move => ??? hf; by inversion hf.
+Defined.
+
+Definition run_v := run_v host_application_impl.
+
+Definition run_step := run_step host_application_impl.
+
+(** State whether a list of administrative instruction is a final value. **)
+Definition is_const_list : list administrative_instruction -> option (list value) :=
+  @those_const_list.
+
+End Interpreter_func.
+
