theories/interpreter_func_extraction_fib.v
@@ -1,0 +1,172 @@
+From mathcomp Require Import eqtype seq ssrfun.
+From Coq Require Import Program.Equality ZArith_base Extraction.
+From Wasm Require Export interpreter_func pp.
+
+Module Extr.
+
+Let host_eqType := unit_eqType.
+
+Definition host : Type := host unit_eqType.
+
+Definition host_instance : host.
+Proof.
+  refine {|
+    host_state := unit_eqType ;
+    host_application _ _ _ _ _ _ _ := False
+  |}; intros; exfalso; auto.
+Defined.
+
+Let store_record := store_record EmptyHost.host_function_eqType.
+Let host_state := host_state EmptyHost.host_instance.
+Let res_tuple := res_tuple EmptyHost.host_instance.
+Let config_tuple := config_tuple EmptyHost.host_instance.
+
+Definition run_step := @run_step _ _ Interpreter_func.host_application_impl.
+Definition run_v := @run_v _ _ Interpreter_func.host_application_impl.
+
+Definition run_v_wrap fuel depth s f es :=
+  let cfg := (tt, s, f, es) in
+  run_v fuel depth cfg.
+
+Check run_v_wrap.
+
+Definition pp_res_val (r : host_state * store_record * res) :=
+  match r with
+  | (_, _, R_value [:: v]) => pp_value v
+  | _ => String.EmptyString
+  end.
+
+Definition i64_of_Z (z: Z) := VAL_int64 (Wasm_int.int_of_Z i64m z).
+
+(*  (func $fibi (param $n i64) (result i64)
+ *    (local $i i64)
+ *    (local $x i64)
+ *    (local $y i64)
+ *    (local $tmp i64)
+ *    (local.set $i (i64.const 0))
+ *    (local.set $x (i64.const 0))
+ *    (local.set $y (i64.const 1))
+ *    (; i is a loop counter ;)
+ *    (; x is 0th, y is 1st fib num ;)
+ *
+ *    (if (i64.eq (local.get $n) (i64.const 0))
+ *     (then (return (i64.const 0)))
+ *    )
+ *
+ *    (loop $loop
+ *      (local.set $i (i64.add (local.get $i) (i64.const 1)))
+ *      (local.set $tmp (i64.add (local.get $x) (local.get $y)))
+ *      (local.set $x (local.get $y))
+ *      (local.set $y (local.get $tmp))
+ *
+ *      (; if $i is less than $n loop again ;)
+ *      (br_if $loop (i64.lt_s (local.get $i) (local.get $n)))
+ *    )
+ *
+ *    (local.get $x)
+ *  )
+ * locals:
+ *   $n: 0
+ *   $i: 1
+ *   $x: 2
+ *   $y: 3
+ * $tmp: 4
+ *)
+
+Let n : Z := 10.
+
+Definition loop_body : seq basic_instruction := [::
+  (* i += 1 *)
+  BI_get_local 1;
+  BI_const (i64_of_Z 1);
+  BI_binop T_i64 (Binop_i BOI_add);
+  BI_set_local 1;
+
+  (* tmp = x + y *)
+  BI_get_local 2;
+  BI_get_local 3;
+  BI_binop T_i64 (Binop_i BOI_add);
+  BI_set_local 4;
+
+  (* x = y *)
+  BI_get_local 3;
+  BI_set_local 2;
+
+  (* y = tmp *)
+  BI_get_local 4;
+  BI_set_local 3;
+
+  (* i < n *)
+  BI_get_local 1;
+  BI_get_local 0;
+  BI_relop T_i64 (Relop_i (ROI_lt SX_S));
+  BI_br_if 0
+].
+
+Definition fib_bis : seq basic_instruction := [::
+  (* n = 10 *)
+  BI_const (i64_of_Z n);
+  BI_set_local 0;
+
+  (* i = 0 *)
+  BI_const (i64_of_Z 0);
+  BI_set_local 1;
+
+  (* x = 0 *)
+  BI_const (i64_of_Z 0);
+  BI_set_local 2;
+
+  (* y = 1 *)
+  BI_const (i64_of_Z 1);
+  BI_set_local 3;
+
+  (* n == 0 *)
+  BI_get_local 0;
+  BI_testop T_i64 TO_eqz;
+  (* (if (i64.eq (local.get $n) (i64.const 0)) *)
+  BI_if
+    (Tf [::] [::T_i64])
+    (* then *)
+    [:: BI_const (i64_of_Z 0)]
+    (* else *)
+    [:: BI_loop (Tf [::] [::]) loop_body; BI_get_local 2]
+].
+
+Definition fib : seq administrative_instruction := map AI_basic fib_bis.
+
+Let emp_store_record : store_record := {|
+  s_funcs   := [::];
+  s_tables  := [::];
+  s_mems    := [::];
+  s_globals := [::];
+|}.
+
+Let emp_instance : instance := {|
+  inst_types  := [::];
+  inst_funcs  := [::];
+  inst_tab    := [::];
+  inst_memory := [::];
+  inst_globs  := [::];
+|}.
+
+Let loc_frame : frame := {|
+  f_locs := [::i64_of_Z 0; i64_of_Z 0; i64_of_Z 0; i64_of_Z 0; i64_of_Z 0];
+  f_inst := emp_instance;
+|}.
+
+(* TODO use Z for fuel *)
+Definition fuel_fib : nat := Z.to_nat (Z.mul (Z.add n 1) 20).
+Definition depth : nat := 10.
+
+End Extr.
+
+(* Check (Extr.run_v Extr.emp_store_record Extr.loc_frame Extr.fib Extr.fuel_fib). *)
+
+From Coq Require Import
+  extraction.ExtrOcamlBasic
+  extraction.ExtrOcamlString.
+
+Extraction Language OCaml.
+
+Extraction "itp_extr" Extr DummyHost.
+
